ROBINSON_PlusPlus/Meta.lean
@@ -80,6 +80,7 @@ import ROBINSON_PlusPlus.Meta.LineWFCases
 import ROBINSON_PlusPlus.Meta.LineWFTrackedPrf
 import ROBINSON_PlusPlus.Meta.InAxiomsCodePrf
 import ROBINSON_PlusPlus.Meta.LineWFThyPrf
+import ROBINSON_PlusPlus.Meta.LineWFMpPrf
 import ROBINSON_PlusPlus.Meta.DiagonalTwo
 import ROBINSON_PlusPlus.Meta.OmegaReflect
 import ROBINSON_PlusPlus.Meta.GodelTwo
